unused.v
@@ -1,3 +1,279 @@
+Lemma concat_empty_l : forall (A:Set) (E:env A),
+  empty & E = E.
+Proof.
+  unfold concat, empty. intros; rewrite* <- app_nil_end.
+Qed.
+
+Lemma incl_map : forall (A:Set) (f:A->A) E1 E2,
+  incl E1 E2 -> incl (map f E1) (map f E2).
+Proof.
+  intros; intro; intros.
+  destruct a.
+  destruct (in_map_inv _ _ _ _ H0) as [b [HE B]].
+  subst.
+  rewrite <- map_snd_env_map.
+  apply (in_map (fun p:var*A => (fst p, f (snd p))) _ _ (H _ B)).
+Qed.
+
+Lemma math_ind : forall Q : nat -> Prop,
+  (forall n, (forall m, m < n -> Q m) -> Q n) ->
+  forall m, Q m.
+Proof.
+  intros.
+  pose (n:= S m).
+  assert (m < n). unfold n; omega.
+  clearbody n.
+  generalize dependent m.
+  induction n; intros.
+    elimtype False; omega.
+  apply H.
+  intros; apply IHn.
+  omega.
+Qed.
+
+Lemma typ_fv_subst_keep : forall S T,
+  typ_fv T << typ_fv (typ_subst S T) \u dom S.
+Proof.
+  induction T; simpl; sets_solve.
+  case_eq (get y S); introv R1.
+    use (binds_dom R1).
+  simpl*.
+Qed.
+
+Lemma fv_in_typ_subst : forall S S0,
+  fv_in typ_fv S0 << fv_in typ_fv (map (typ_subst S) S0) \u dom S.
+Proof.
+  induction S0; simpl; intros y Hy. auto.
+  destruct a. simpl.
+  sets_solve.
+  use (typ_fv_subst_keep S t).
+Qed.
+
+Lemma kind_fv_subst_keep : forall S k,
+  kind_fv k << kind_fv (kind_subst S k) \u dom S.
+Proof.
+  unfold kind_fv; destruct k as [[kc kv kr kh]|]; simpl*.
+  clear kh; induction kr; simpl*.
+  use (typ_fv_subst_keep S (snd a)).
+Qed.
+
+Lemma fv_in_remove_env : forall (A:Set) fv v (a:A) E,
+  binds v a E ->
+  fv_in fv E << fv a \u fv_in fv (remove_env E v).
+Proof.
+  unfold binds; induction E; simpl; intros. discriminate.
+  destruct a0.
+  destruct (v == v0).
+    inversions* H.
+  simpl*.
+Qed.
+
+Lemma remove_env_idem : forall (A:Set) v (E:env A),
+  v # E -> remove_env E v = E.
+Proof.
+  induction E; simpl; intros. auto.
+  destruct a.
+  destruct (v == v0).
+    elim H; subst*.
+  rewrite* IHE.
+Qed.
+
+Lemma kind_fv_in_remove_env : forall v E,
+  fv_in kind_fv E << kind_fv (get_kind v E) \u fv_in kind_fv (remove_env E v).
+Proof.
+  intros.
+  unfold get_kind.
+  case_eq (get v E); intros.
+    apply* fv_in_remove_env.
+  use (get_none_notin _ H).
+  rewrite* (remove_env_idem _ H0).
+Qed.
+
+Lemma unify_keep_fv : forall K S E h pairs K0 S0,
+  Body.unify h pairs K0 S0 = Some (K, S) ->
+  is_subst S0 -> ok K0 ->
+  fvs S0 K0 E << fvs S K E.
+Proof.
+  intros until 2.
+  apply* (unify_ind (K':=K) (S':=S)
+    (fun K0 S0 _ => ok K0 -> fvs S0 K0 E << fvs S K E));
+    clear H H0 K0 S0 pairs h.
+    intros until K1.
+    unfold K1, S1, fvs; clear K1 S1.
+    intros _ R1 R2 _ _ _ R4 IH HK0 y Hy.
+    apply* IH; clear IH.
+    unfold compose.
+    rewrite dom_concat. rewrite* dom_remove_env.
+    rewrite dom_map. rewrite fv_in_concat.
+    simpl dom.
+    sets_solve.
+        puts (fv_in_typ_subst (v ~ T) _ H0); simpl in *. sets_solve.
+      destruct (v == y); subst*.
+    use (kind_fv_in_remove_env v _ H0).
+    rewrite R4 in H.
+    replace (kind_fv None) with {} in H by reflexivity.
+    auto.
+  intros until K1.
+  unfold K1, S1, fvs; clear K1 S1.
+  intros R3 HU _ _ _ HSv n IH HK0.
+  assert (ok (remove_env (remove_env K0 v) v0 & v0 ~ k)).
+    apply* ok_push.
+    rewrite* dom_remove_env.
+  poses HS (IH H); clear IH H.
+  unfold compose in HS. repeat rewrite dom_concat in HS.
+  rewrite dom_map in HS. repeat rewrite fv_in_concat in HS.
+  simpl in HS. simpl.
+  do 2 rewrite dom_remove_env in HS; auto.
+  sets_solve.
+      apply HS.
+      use (fv_in_typ_subst (v ~ typ_fvar v0) _ H0).
+      simpl in H; auto.
+    apply HS.
+    destruct (v == y). subst*.
+    destruct* (v0 == y). subst*.
+  poses Hun (unify_types _ _ _ HU HSv).
+  destruct (unify_kinds_sound _ _ (S:=S) R3).
+    intro; intros. apply* Hun.
+  puts (kind_fv_in_remove_env v _ H0).
+  clear H0 Hun; sets_solve.
+    use (kind_fv_subst_keep S _ H0).
+    sets_solve.
+    use (kind_entails_fv _ _ H H3).
+    use (kind_fv_subst _ _ H2).
+  puts (kind_fv_in_remove_env v0 _ H0).
+  clear H H0 R3; sets_solve.
+  unfold get_kind in *.
+  case_rewrite (get v0 K0) R3.
+    rewrite (binds_remove_env (v:=v) R3) in H.
+      use (kind_fv_subst_keep S _ H); clear H.
+      sets_solve.
+      puts (kind_entails_fv _ _ H1 H).
+      use (kind_fv_subst _ _ H0).
+    auto*.
+  rewrite get_notin_dom in H. elim (in_empty H).
+  rewrite* dom_remove_env.
+  intro. elim (get_none_notin _ R3). auto.
+Qed.
+
+Lemma diff_union_l : forall L1 L2 L3,
+  S.diff (L1 \u L2) L3 = S.diff L1 L3 \u S.diff L2 L3.
+Proof.
+  intros.
+  apply eq_ext; intro; split; intros; auto.
+Qed.
+
+Lemma unify_complete' : forall S0 K0 S K T1 T2,
+  is_subst S0 -> ok K0 -> extends S S0 ->
+  typ_subst S T1 = typ_subst S T2 ->
+  well_subst K0 K S ->
+  exists K', exists S',
+    unify K0 T1 T2 S0 = Some (K', S') /\ extends S S' /\ well_subst K' K S.
+Proof.
+  intros.
+  assert (unifies S ((T1,T2)::nil)).
+    intro; simpl; intros. destruct* H4; inversions* H4.
+  case_eq (unify K0 T1 T2 S0); unfold unify; intros.
+    destruct p as [K' S']. esplit; esplit; split*.
+    apply* (unify_mgu0 _ H5 (K':=K) (S':=S)).
+  elimtype False.
+  refine (unify_complete0 (K:=K) (S:=S) _ _ _ _ _ _ H5); auto.
+Qed.
+
+Lemma fv_subset_abs : forall S K E T Ts X1 X2 x,
+  unifies S ((typ_arrow X1 X2, T) :: nil) ->
+  fvs S K E T Ts = fvs S K ((x, Sch X1 nil) :: E) X2 (T::Ts).
+Proof.
+  intros.
+  unfold fvs, env_fv; simpl.
+  apply eq_ext; intro y; simpl; split*.
+  unfold sch_fv.
+  simpl.
+  intro Hy; sets_solve;
+    assert (y \in typ_fv (typ_arrow X1 X2)) by (simpl; auto with sets);
+    use (typ_fv_subst_keep S _ H0);
+    rewrite (H (typ_arrow X1 X2) T) in H2; simpl*;
+    destruct* (S.union_1 H2); clear H0 H1 H2;
+    use (typ_fv_subst _ _ H3).
+Qed.
+
+Lemma unifies_extends : forall S1 S2 l,
+  unifies S1 l -> extends S2 S1 -> unifies S2 l.
+Proof.
+  intros; intro; intros.
+  rewrite <- (H0 T1); rewrite <- (H0 T2).
+  apply (f_equal (typ_subst S2)).
+  apply* H.
+Qed.
+
+Lemma ok_map_inv : forall (A:Set) (f:A->A) E, ok (map f E) -> ok E.
+Proof.
+  induction E; intro. auto.
+  destruct a. simpl in H. inversions H.
+  apply* ok_cons.
+Qed.
+
+Lemma combine_For_all2 : forall (A B:Set) (P:A->B->Prop) l1 l2,
+  length l1 = length l2 ->
+  (forall a b, In (a,b) (combine l1 l2) -> P a b) ->
+  For_all2 P l1 l2.
+Proof.
+  induction l1; destruct l2; simpl; intros; try discriminate; auto*.
+Qed.
+
+Lemma list_map_combine_swap : forall (A B C D:Set) (f1:A->C) (f2:B->D) l1 l2,
+  List.map (fun p:A*B => (f2 (snd p), f1 (fst p))) (combine l1 l2) =
+  combine (List.map f2 l2) (List.map f1 l1).
+Proof.
+  induction l1; destruct l2; simpl; intros; auto.
+  rewrite* IHl1.
+Qed.
+
+Lemma well_subst_For_all2: forall K Ks Xs Vs,
+  well_subst (K & kinds_open_vars Ks Xs) K (combine Xs Vs) ->
+  fresh (kind_fv_list Ks) (length Ks) Xs ->
+  types (length Xs) Vs ->
+  For_all2 (well_kinded K) (kinds_open Ks Vs) Vs.
+Proof.
+  introv WS Fr HVs.
+  apply combine_For_all2.
+    unfold kinds_open. rewrite map_length. rewrite (fresh_length _ _ _ Fr).
+    apply (proj1 HVs).
+  intros.
+  replace (combine (kinds_open Ks Vs) Vs) with
+    (List.map (fun p:var*kind =>
+      (kind_subst (combine Xs Vs) (snd p),
+       typ_subst (combine Xs Vs) (typ_fvar (fst p)))) (kinds_open_vars Ks Xs))
+    in H.
+    destruct (proj1 (in_map_iff _ _ _) H) as [[x k] [HE HB]].
+    simpl in HE; inversions HE; clear HE H.
+    apply (WS x).
+    apply binds_prepend.
+    apply* in_ok_binds.
+    unfold kinds_open_vars. apply* ok_combine_fresh.
+  unfold kinds_open_vars.
+  rewrite (list_map_combine_swap
+    (fun x => typ_subst (combine Xs Vs) (typ_fvar x))
+    (kind_subst (combine Xs Vs))).
+  rewrite <- (map_map typ_fvar (typ_subst (combine Xs Vs))).
+  rewrite kinds_subst_open.
+    rewrite <- (fresh_length _ _ _ Fr) in HVs.
+    rewrite (proj1 HVs) in Fr.
+    fold (typ_fvars Xs).
+    rewrite (fresh_subst _ _ _ Fr).
+    rewrite (list_map_ext Ks (kind_subst (combine Xs Vs)) (fun k => k)).
+      rewrite* list_map_id.
+    intros.
+    use (in_kind_fv _ _ H0).
+    rewrite* kind_subst_fresh.
+    rewrite dom_combine.
+      apply disjoint_comm.
+      apply (fresh_disjoint (length Vs)).
+      apply* fresh_sub.
+    rewrite* (fresh_length _ _ _ Fr).
+  apply* list_forall_env_prop.
+  apply (proj2 HVs).
+Qed.
+
 Lemma elements_mkset : forall l,
   sort S.E.lt l -> S.elements (mkset l) = l.
 Proof.
@@ -103,3 +379,194 @@ Proof.
   use (IHF _ _ H).
 Qed.
 
+Lemma unify_idem : forall K S h pairs,
+  unifies S pairs ->
+  is_subst S ->
+  h > size_pairs S K pairs ->
+  Body.unify h pairs K S = Some (K, S).
+Proof.
+  induction h using math_ind; intros.
+  destruct h.
+    elimtype False; omega.
+  destruct pairs.
+    simpl*.
+  destruct p; simpl.
+  assert (typ_subst S t = typ_subst S t0)
+    by (unfold unifies in H0; apply* H0).
+  use (size_pairs_grows S K (t,t0) pairs).
+  assert (unifies S pairs) by (unfold unifies in *; intros; apply* H0).
+  case_eq (typ_subst S t); introv R1; rewrite H3 in R1; rewrite R1.
+      destruct* (n === n). apply* H. omega.
+    destruct* (v == v). apply* H. omega.
+  assert (size_pairs S K ((t1, t1) :: (t2, t2) :: pairs) <
+          size_pairs S K ((t, t0) :: pairs)).
+    unfold size_pairs, all_size, really_all_fv, all_fv.
+    simpl.
+    rewrite <- (typ_subst_idem t H1).
+    rewrite <- (typ_subst_idem t0 H1).
+    rewrite H3.
+    rewrite R1; simpl.
+    apply pow2exp_lt_le.
+      omega.
+    assert (forall b a c, a \u (b \u c) = b \u (a \u c)).
+      intros. rewrite union_assoc. rewrite (union_comm a).
+      rewrite* <- union_assoc.
+    rewrite (H6 (typ_fv (typ_subst S t2))).
+    repeat rewrite union_assoc.
+    omega.
+  apply* H.
+    intro; simpl; intros. destruct H7. inversions* H7.
+    destruct H7. inversions* H7.
+    apply* (H5 T1).
+  omega.
+Qed.
+
+Section Unique_Env.
+Variable (A:Set).
+
+Fixpoint make_ok (L:vars) (E:env A) {struct E} : env A :=
+  match E with
+  | nil => nil
+  | a :: E' =>
+    if S.mem (fst a) L then make_ok L E'
+    else a :: make_ok (S.add (fst a) L) E'
+  end.
+
+Lemma make_ok_ok : forall E,
+  let E' := make_ok {} E in
+  incl E E' /\ incl E' E /\ ok E'.
+Proof.
+  intros.
+  set (L := {}) in E'.
+  assert (ok E' /\ disjoint L (dom E') /\
+          forall x, x \notin L -> get x E = get x E').
+    unfold E'; clear E'.
+    gen L; induction E; intros.
+      simpl. intuition.
+        fold (@empty A). apply ok_empty.
+      intro; auto.
+    destruct a.
+    simpl in *.
+    case_eq (S.mem v L); intros; simpl.
+      destruct (IHE L).
+      intuition.
+      destruct* (x == v).
+      subst.
+      elim H1; apply* S.mem_2.
+    destruct (IHE (S.add v L)).
+    intuition.
+        apply* ok_cons.
+        destruct* (H2 v).
+        elim H1; auto with sets.
+      disjoint_solve.
+        left; intro. elim H1; auto with sets.
+      destruct* (v == v0).
+      subst.
+      use (mem_3 H).
+    destruct* (x == v).
+    apply H3.
+    intro; elim H1. apply* S.add_3.
+  intuition; intro; intros.
+    unfold binds; rewrite* <- (H2 x).
+    intro. elim (in_empty H3).
+  unfold binds; rewrite* (H2 x).
+  intro. elim (in_empty H3).
+Qed.
+End Unique_Env.
+
+Definition non_self_binding (p:var*typ) :=
+  let (x,a) := p in
+  match a with
+  | typ_fvar y => if x == y then false else true
+  | _ => true
+  end.
+
+Lemma filter_env_ok : forall (A:Set) f (E:env A),
+  ok E -> ok (filter f E).
+Proof.
+  intros.
+  apply (proj2 (A:=dom (filter f E) << dom E)).
+  induction H; intros. simpl.
+     split*. fold (@empty A); auto.
+  simpl.
+  case_eq (f (@pair var A x a)); intros.
+    split. simpl.
+      destruct* IHok.
+    apply* ok_cons.
+  split*.
+Qed.
+
+Lemma binds_filter : forall (A:Set) f x (a:A) E,
+  binds x a (filter f E) -> ok E -> binds x a E /\ f (x,a) = true.
+Proof.
+  intros.
+  poses Hin (binds_in H).
+  destruct (proj1 (filter_In _ _ _) Hin).
+  use (in_ok_binds _ _ H1 H0).
+Qed.
+
+Lemma typ_subst_eq_ind : forall S1 S2,
+  (forall x, typ_subst S1 (typ_fvar x) = typ_subst S2 (typ_fvar x)) ->
+  forall T, typ_subst S1 T = typ_subst S2 T.
+Proof.
+  induction T; auto. simpl; congruence.
+Qed.
+
+Definition ext_subst S :=
+  forall x,
+    x \notin fv_in typ_fv S \/ typ_subst S (typ_fvar x) = typ_fvar x.
+
+Lemma is_subst_dom : forall S x,
+  is_subst S ->  ~ binds x (typ_fvar x) S.
+Proof.
+  intros; intro.
+  use (binds_dom H0).
+  destruct* (H _ _ H0 x).
+  simpl in H2.
+  notin_contradiction.
+Qed.
+
+Lemma ext_subst_is_subst : forall S,
+  ext_subst S ->
+  exists S', is_subst S' /\ forall T, typ_subst S T = typ_subst S' T.
+Proof.
+  unfold ext_subst; intros.
+  destruct (make_ok_ok S).
+  destruct H1.
+  set (S0 := make_ok {} S) in *.
+  exists (filter non_self_binding S0).
+  assert (is_subst (filter non_self_binding S0)).
+    intro; intros.
+    destruct* (binds_filter _ H3).
+    use (H1 _ _ H4).
+    intro y.
+    destruct (H y).
+      use (fv_in_spec typ_fv H6).
+    simpl in H7.
+    left.
+    case_eq (get y (filter non_self_binding S0)); introv R1.
+      destruct* (binds_filter _ R1).
+      use (H1 _ _ H8).
+      rewrite H10 in H7.
+      subst. simpl in H9.
+      destruct* (y == y). discriminate.
+    apply (get_none_notin _ R1).
+  split*.
+  apply typ_subst_eq_ind.
+  intro; simpl.
+  case_eq (get x (filter non_self_binding S0)); introv R1.
+    destruct* (binds_filter _ R1).
+    rewrite* (H1 _ _ H4).
+  destruct (H x).
+    case_eq (get x S); introv R2; auto.
+    use (binds_in (H0 _ _ R2)).
+    case_eq (non_self_binding (x,t)); introv R3.
+      use (proj2 (filter_In _ _ _) (conj H5 R3)).
+      rewrite (in_ok_binds _ _ H6 (filter_env_ok _ H2)) in R1.
+      discriminate.
+    simpl in R3.
+    destruct t; try discriminate.
+    destruct (x == v); try discriminate.
+    subst*.
+  apply H4.
+Qed.
